backend/Constpropproof.v
@@ -33,7 +33,7 @@ Proof.
 Qed.
 
 Definition match_pol (prog: program) :=
-  Policy.match_pol (fun cu f tf => tf = transf_fundef (romem_for cu) f) prog.
+  match_pol_gen (fun cu f tf => tf = transf_fundef (romem_for cu) f) prog.
 
 Section PRESERVATION.
 
@@ -46,8 +46,8 @@ Hypothesis TRANSPOL: match_pol prog pol tpol.
 
 Lemma linkorder_policy:
   forall cunit, linkorder cunit prog ->
-           Policy.match_pol (fun cu f tf => tf = transf_fundef (romem_for cu) f) prog pol tpol ->
-           Policy.match_pol (fun cu f tf => tf = transf_fundef (romem_for cu) f) cunit pol tpol.
+           match_pol_gen (fun cu f tf => tf = transf_fundef (romem_for cu) f) prog pol tpol ->
+           match_pol_gen (fun cu f tf => tf = transf_fundef (romem_for cu) f) cunit pol tpol.
 Admitted.
 
 Let ge := Genv.globalenv prog.
