backend/Deadcodeproof.v
@@ -384,7 +384,7 @@ Proof.
   + apply eagree_update; auto with na.
 Qed.
 
-Definition match_pol (prog: program) := Policy.match_pol (fun cu f tf => OK tf = transf_fundef (romem_for cu) f) prog.
+Definition match_pol (prog: program) := match_pol_gen (fun cu f tf => OK tf = transf_fundef (romem_for cu) f) prog.
 
 (** * Basic properties of the translation *)
 
@@ -399,8 +399,8 @@ Hypothesis TRANSPOL: match_pol prog pol tpol.
 
 Lemma linkorder_policy:
   forall cunit, linkorder cunit prog ->
-           Policy.match_pol (fun cu f tf => OK tf = transf_fundef (romem_for cu) f) prog pol tpol ->
-           Policy.match_pol (fun cu f tf => OK tf = transf_fundef (romem_for cu) f) cunit pol tpol.
+           match_pol_gen (fun cu f tf => OK tf = transf_fundef (romem_for cu) f) prog pol tpol ->
+           match_pol_gen (fun cu f tf => OK tf = transf_fundef (romem_for cu) f) cunit pol tpol.
 Admitted.
 
 Let ge := Genv.globalenv prog.
